

05.11.25

~~$$\dot{x} = f(x) + g(x)u - \varphi(x)\mu$$~~

КАК ОСУЩЕСТВ. КОМПЕНС.?

~~$$\hat{\mu} : g(x)u - \varphi(x)\hat{\mu} = g(x)u_b$$~~

~~$$u = u_b + u_c$$~~

~~$$g(x)u_b + g(x)u_c - \varphi(x)\hat{\mu} = g(x)u_b$$~~

~~$$g(x)u_c = \varphi(x)\hat{\mu}$$~~

$$\dot{x} = f(x) + g(u) + \varphi^T(x)\mu$$

$\hat{\mu}$ - ОЦЕНКА

// g

$$u = u_b + u_c$$

$$g(u) + \varphi^T(x)\hat{\mu} = g(u_b)$$

$$g(u_b + u_c) = g(u_b) - \varphi^T(x)\hat{\mu}$$

$$u_b + u_c = \bar{g}^{-1}(g(u_b) - \varphi^T(x)\hat{\mu})$$

u_c

ПОДСТАВИМ В УРАВН.

$$\dot{x} = f(x) + \cancel{g}(\bar{g}^{-1}(g(u_b) - \varphi^T(x)\hat{\mu})) + \varphi^T(x)\mu$$

$$\dot{x} = f(x) + g(u_b) + \varphi^T(x)(\mu - \hat{\mu})$$

$$V(x) = \underbrace{V_0(x)}_{CLF} + \frac{(\mu - \hat{\mu})^T(\mu - \hat{\mu})}{2\lambda}$$

$$\begin{aligned} \frac{d}{dt} V(x) &= \nabla V_0^T \dot{x} + \frac{\dot{\hat{\mu}}(\mu - \hat{\mu})}{\lambda} = \nabla V_0^T f(x) + \nabla V_0^T g(u_b) + \\ &+ \nabla V_0^T \varphi^T(x)(\mu - \hat{\mu}) + \frac{\dot{\hat{\mu}}(\mu - \hat{\mu})}{\lambda} = \underbrace{\nabla V_0^T (f(x) + g(u_b))}_{<0} + \\ &+ (\mu - \hat{\mu}) \left[\nabla V_0^T \varphi^T(x) - \frac{\dot{\hat{\mu}}}{\lambda} \right] \leq 0 \end{aligned}$$

ЛИН. СЛУЧАЙ

$$\begin{pmatrix} \dot{p} \\ \ddot{p} \end{pmatrix} = \begin{pmatrix} 0 & 1 \\ 0 & 0 \end{pmatrix} \begin{pmatrix} p \\ \dot{p} \end{pmatrix} + \begin{pmatrix} 0 \\ \frac{1}{m} \end{pmatrix} F$$

$\dot{x} \quad A \quad x \quad B \quad u$

ЗНАЕМ B, u - ?

| $\bar{g}^{-1}(\dots)$

$$\nabla V_0^T \varphi^T(x) = \frac{\hat{u}^T}{2}$$

$$\hat{u}^T = 2 \nabla V_0^T \varphi^T(x)$$

$$\hat{u} = 2 \varphi(x) \nabla V_0$$